all but flushes

lib/Buckets/KVList.i.dfy
@@ -33,14 +33,18 @@ module KVList {
   datatype Kvl = Kvl(keys: PSA.Psa, messages: seq<Message>)
 
   predicate WF(kvl: Kvl) {
-    && PSA.psaNumStrings(kvl.keys) as int == |kvl.messages|
+    && PSA.WF(kvl.keys)
+    && (forall i :: 0 <= i < PSA.psaNumStrings(kvl.keys) ==> |PSA.psaElement(kvl.keys, i)| <= MaxLen() as int)
     && IsStrictlySorted(PSA.I(kvl.keys))
+    && PSA.psaNumStrings(kvl.keys) as int == |kvl.messages|
     && (forall i | 0 <= i < |kvl.messages| :: kvl.messages[i] != IdentityMessage())
   }
 
   function {:opaque} IMap(kvl: Kvl) : BucketMap
+  requires PSA.WF(kvl.keys)
   requires PSA.psaNumStrings(kvl.keys) as int == |kvl.messages|
   ensures PSA.psaNumStrings(kvl.keys) as int == 0 ==> |IMap(kvl).Keys| == 0    // empty input -> empty output.
+  ensures forall k | k in IMap(kvl).Keys :: |k| <= MaxLen() as int
   decreases PSA.psaNumStrings(kvl.keys)
   {
     if PSA.psaNumStrings(kvl.keys) == 0 then map[] else (
@@ -49,12 +53,15 @@ module KVList {
   }
 
   function I(kvl: Kvl) : Bucket
+  requires PSA.WF(kvl.keys)
   requires PSA.psaNumStrings(kvl.keys) as int == |kvl.messages|
+  ensures WF(kvl) ==> forall k | k in I(kvl).b.Keys :: |k| <= MaxLen() as int
   {
     B(IMap(kvl))
   }
 
   function {:opaque} ISeq(kvls: seq<Kvl>) : (s : seq<Bucket>)
+  requires forall i :: 0 <= i < |kvls| ==> PSA.WF(kvls[i].keys)
   requires forall i | 0 <= i < |kvls| :: PSA.psaNumStrings(kvls[i].keys) as int == |kvls[i].messages|
   ensures |s| == |kvls|
   ensures forall i | 0 <= i < |kvls| :: s[i] == I(kvls[i])
@@ -63,10 +70,11 @@ module KVList {
   }
 
   function prefix(kvl: Kvl, i: int) : Kvl
+  requires PSA.WF(kvl.keys)
   requires 0 <= i <= PSA.psaNumStrings(kvl.keys) as int
   requires 0 <= i <= |kvl.messages|
   {
-    Kvl(PSA.psaPrefix(kvl.keys, i as uint64), kvl.messages[..i]) 
+    Kvl(PSA.psaSubSeq(kvl.keys, 0, i as uint64), kvl.messages[..i]) 
   }
 
   lemma WFPrefix(kvl: Kvl, i: int)
@@ -74,10 +82,17 @@ module KVList {
   requires 0 <= i <= PSA.psaNumStrings(kvl.keys) as int
   ensures WF(prefix(kvl, i))
   {
+    var pre := prefix(kvl, i);
+    forall j | 0 <= j < PSA.psaNumStrings(pre.keys)
+      ensures |PSA.psaElement(pre.keys, j)| <= MaxLen() as int
+    {
+      assert PSA.psaElement(pre.keys, j) == PSA.psaElement(kvl.keys, j);
+    }
     reveal_IsStrictlySorted();
   }
 
   lemma IndexOfKey(kvl: Kvl, key: Key) returns (i : int)
+  requires PSA.WF(kvl.keys)
   requires PSA.psaNumStrings(kvl.keys) as int == |kvl.messages|
   requires key in IMap(kvl)
   ensures 0 <= i < PSA.psaNumStrings(kvl.keys) as int
@@ -101,9 +116,10 @@ module KVList {
     reveal_IMap();
     if (i == PSA.psaNumStrings(kvl.keys) as int - 1) {
     } else {
-      reveal_IsStrictlySorted();
+      WFPrefix(kvl, PSA.psaNumStrings(kvl.keys) as int - 1);
       Imaps(Kvl(PSA.psaDropLast(kvl.keys), DropLast(kvl.messages)), i);
-      assert PSA.LastElement(kvl.keys) != PSA.psaElement(kvl.keys, i as uint64);
+      var ikeys := PSA.I(kvl.keys);
+      IsStrictlySortedImpliesLt(ikeys, i, |ikeys|-1);
     }
   }
 
@@ -128,414 +144,428 @@ module KVList {
   /////////////////////////
 
   function append(kvl: Kvl, key: Key, value: Message) : Kvl
+  requires PSA.WF(kvl.keys)
+  requires |kvl.keys.offsets| < 0x1_000_0000 - 1
+  requires |kvl.keys.data| + |key| < 0x1_0000_0000
   {
     Kvl(PSA.psaAppend(kvl.keys, key), kvl.messages + [value])
   }
 
   lemma Iappend(kvl: Kvl, key: Key, value: Message)
+  requires PSA.WF(kvl.keys)
   requires PSA.psaNumStrings(kvl.keys) as int == |kvl.messages|
+  requires |kvl.keys.offsets| < 0x1_000_0000 - 1
+  requires |kvl.keys.data| + |key| < 0x1_0000_0000
   ensures IMap(append(kvl, key, value)) == IMap(kvl)[key := value]
   {
     reveal_IMap();
+    var app := append(kvl, key, value);
+    assert PSA.LastElement(app.keys) == key;
   }
 
   lemma Iprefix_append(kvl: Kvl, i: int)
+  requires PSA.WF(kvl.keys)
   requires PSA.psaNumStrings(kvl.keys) as int == |kvl.messages|
+  requires |kvl.keys.offsets| < 0x1_000_0000
   requires 0 <= i < PSA.psaNumStrings(kvl.keys) as int
+  requires forall j :: 0 <= j < PSA.psaNumStrings(kvl.keys) ==> |PSA.psaElement(kvl.keys, j as uint64)| <= MaxLen() as int
   ensures IMap(prefix(kvl, i + 1)) == IMap(prefix(kvl, i))[PSA.psaElement(kvl.keys, i as uint64) := kvl.messages[i]]
   {
     assert prefix(kvl, i + 1) == append(prefix(kvl, i), PSA.psaElement(kvl.keys, i as uint64), kvl.messages[i]);
     Iappend(prefix(kvl, i), PSA.psaElement(kvl.keys, i as uint64), kvl.messages[i]);
   }
 
-  function flushIterate(parent: Kvl, children: seq<Kvl>, pivots: seq<Key>,
-      parentIdx: int, childrenIdx: int, childIdx: int, acc: seq<Kvl>, cur: Kvl) : seq<Kvl>
-  requires WF(parent)
-  requires forall i | 0 <= i < |children| :: WF(children[i])
-  requires |pivots| + 1 == |children|
-  requires 0 <= parentIdx <= PSA.psaNumStrings(parent.keys) as int
-  requires 0 <= childrenIdx <= |children|
-  requires childrenIdx < |children| ==> 0 <= childIdx <= PSA.psaNumStrings(children[childrenIdx].keys) as int
-  decreases |children| - childrenIdx
-  decreases PSA.psaNumStrings(parent.keys) as int - parentIdx +
-      (if childrenIdx < |children| then PSA.psaNumStrings(children[childrenIdx].keys) as int - childIdx else 0)
-  {
-    if childrenIdx == |children| then (
-      acc
-    ) else (
-      var child := children[childrenIdx];
+  // function flushIterate(parent: Kvl, children: seq<Kvl>, pivots: seq<Key>,
+  //     parentIdx: int, childrenIdx: int, childIdx: int, acc: seq<Kvl>, cur: Kvl) : seq<Kvl>
+  // requires WF(parent)
+  // requires forall i | 0 <= i < |children| :: WF(children[i])
+  // requires |pivots| + 1 == |children|
+  // requires 0 <= parentIdx <= PSA.psaNumStrings(parent.keys) as int
+  // requires 0 <= childrenIdx <= |children|
+  // requires childrenIdx < |children| ==> 0 <= childIdx <= PSA.psaNumStrings(children[childrenIdx].keys) as int
+  // requires |cur.keys.offsets| < 0x1_000_0000 - 1
+  // requires |cur.keys.data| + |key| < 0x1_0000_0000
+  // decreases |children| - childrenIdx
+  // decreases PSA.psaNumStrings(parent.keys) as int - parentIdx +
+  //     (if childrenIdx < |children| then PSA.psaNumStrings(children[childrenIdx].keys) as int - childIdx else 0)
+  // {
+  //   if childrenIdx == |children| then (
+  //     acc
+  //   ) else (
+  //     var child := children[childrenIdx];
 
-      if parentIdx == PSA.psaNumStrings(parent.keys) as int then (
-        if childIdx == PSA.psaNumStrings(child.keys) as int then (
-          flushIterate(parent, children, pivots, parentIdx, childrenIdx + 1, 0, acc + [cur], Kvl(PSA.EmptyPsa(), []))
-        //) else if |cur.keys| == 0 then (
-        //  flushIterate(parent, children, pivots, parentIdx, childrenIdx + 1, 0, acc + [child], Kvl(PSA.EmptyPsa(), []))
-        ) else (
-          flushIterate(parent, children, pivots, parentIdx, childrenIdx, childIdx + 1, acc, append(cur, PSA.psaElement(child.keys, childIdx as uint64), child.messages[childIdx]))
-        )
-      ) else (
-        if childIdx == PSA.psaNumStrings(child.keys) as int then (
-          if childrenIdx == |children| - 1 then (
-            flushIterate(parent, children, pivots, parentIdx + 1, childrenIdx, childIdx, acc, append(cur, PSA.psaElement(parent.keys, parentIdx as uint64), parent.messages[parentIdx]))
-          ) else (
-            if lt(PSA.psaElement(parent.keys, parentIdx as uint64), pivots[childrenIdx]) then (
-              flushIterate(parent, children, pivots, parentIdx + 1, childrenIdx, childIdx, acc, append(cur, PSA.psaElement(parent.keys, parentIdx as uint64), parent.messages[parentIdx]))
-            ) else (
-              flushIterate(parent, children, pivots, parentIdx, childrenIdx + 1, 0, acc + [cur], Kvl(PSA.EmptyPsa(), []))
-            )
-          )
-        ) else (
-          if PSA.psaElement(child.keys, childIdx as uint64) == PSA.psaElement(parent.keys, parentIdx as uint64) then (
-            var m := Merge(parent.messages[parentIdx], child.messages[childIdx]);
-            if m == IdentityMessage() then (
-              flushIterate(parent, children, pivots, parentIdx + 1, childrenIdx, childIdx + 1, acc, cur)
-            ) else (
-              flushIterate(parent, children, pivots, parentIdx + 1, childrenIdx, childIdx + 1, acc, append(cur, PSA.psaElement(child.keys, childIdx as uint64), m))
-            )
-          ) else if lt(PSA.psaElement(child.keys, childIdx as uint64), PSA.psaElement(parent.keys, parentIdx as uint64)) then (
-            flushIterate(parent, children, pivots, parentIdx, childrenIdx, childIdx + 1, acc, append(cur, PSA.psaElement(child.keys, childIdx as uint64), child.messages[childIdx]))
-          ) else (
-            flushIterate(parent, children, pivots, parentIdx + 1, childrenIdx, childIdx, acc, append(cur, PSA.psaElement(parent.keys, parentIdx as uint64), parent.messages[parentIdx]))
-          )
-        )
-      )
-    )
-  }
+  //     if parentIdx == PSA.psaNumStrings(parent.keys) as int then (
+  //       if childIdx == PSA.psaNumStrings(child.keys) as int then (
+  //         flushIterate(parent, children, pivots, parentIdx, childrenIdx + 1, 0, acc + [cur], Kvl(PSA.EmptyPsa(), []))
+  //       //) else if |cur.keys| == 0 then (
+  //       //  flushIterate(parent, children, pivots, parentIdx, childrenIdx + 1, 0, acc + [child], Kvl(PSA.EmptyPsa(), []))
+  //       ) else (
+  //         flushIterate(parent, children, pivots, parentIdx, childrenIdx, childIdx + 1, acc, append(cur, PSA.psaElement(child.keys, childIdx as uint64), child.messages[childIdx]))
+  //       )
+  //     ) else (
+  //       if childIdx == PSA.psaNumStrings(child.keys) as int then (
+  //         if childrenIdx == |children| - 1 then (
+  //           flushIterate(parent, children, pivots, parentIdx + 1, childrenIdx, childIdx, acc, append(cur, PSA.psaElement(parent.keys, parentIdx as uint64), parent.messages[parentIdx]))
+  //         ) else (
+  //           if lt(PSA.psaElement(parent.keys, parentIdx as uint64), pivots[childrenIdx]) then (
+  //             flushIterate(parent, children, pivots, parentIdx + 1, childrenIdx, childIdx, acc, append(cur, PSA.psaElement(parent.keys, parentIdx as uint64), parent.messages[parentIdx]))
+  //           ) else (
+  //             flushIterate(parent, children, pivots, parentIdx, childrenIdx + 1, 0, acc + [cur], Kvl(PSA.EmptyPsa(), []))
+  //           )
+  //         )
+  //       ) else (
+  //         if PSA.psaElement(child.keys, childIdx as uint64) == PSA.psaElement(parent.keys, parentIdx as uint64) then (
+  //           var m := Merge(parent.messages[parentIdx], child.messages[childIdx]);
+  //           if m == IdentityMessage() then (
+  //             flushIterate(parent, children, pivots, parentIdx + 1, childrenIdx, childIdx + 1, acc, cur)
+  //           ) else (
+  //             flushIterate(parent, children, pivots, parentIdx + 1, childrenIdx, childIdx + 1, acc, append(cur, PSA.psaElement(child.keys, childIdx as uint64), m))
+  //           )
+  //         ) else if lt(PSA.psaElement(child.keys, childIdx as uint64), PSA.psaElement(parent.keys, parentIdx as uint64)) then (
+  //           flushIterate(parent, children, pivots, parentIdx, childrenIdx, childIdx + 1, acc, append(cur, PSA.psaElement(child.keys, childIdx as uint64), child.messages[childIdx]))
+  //         ) else (
+  //           flushIterate(parent, children, pivots, parentIdx + 1, childrenIdx, childIdx, acc, append(cur, PSA.psaElement(parent.keys, parentIdx as uint64), parent.messages[parentIdx]))
+  //         )
+  //       )
+  //     )
+  //   )
+  // }
 
-  function flush(parent: Kvl, children: seq<Kvl>, pivots: seq<Key>) : seq<Kvl>
-  requires WF(parent)
-  requires forall i | 0 <= i < |children| :: WF(children[i])
-  requires |pivots| + 1 == |children|
-  {
-    flushIterate(parent, children, pivots, 0, 0, 0, [], Kvl(PSA.EmptyPsa(), []))
-  }
+  // function flush(parent: Kvl, children: seq<Kvl>, pivots: seq<Key>) : seq<Kvl>
+  // requires WF(parent)
+  // requires forall i | 0 <= i < |children| :: WF(children[i])
+  // requires |pivots| + 1 == |children|
+  // {
+  //   flushIterate(parent, children, pivots, 0, 0, 0, [], Kvl(PSA.EmptyPsa(), []))
+  // }
 
-  predicate flushIterateInv(parent: Kvl, children: seq<Kvl>, pivots: seq<Key>,
-      parentIdx: int, childrenIdx: int, childIdx: int, acc: seq<Kvl>, cur: Kvl)
-  {
-    && WF(parent)
-    && (forall i | 0 <= i < |children| :: WF(children[i]))
-    && WFBucketListProper(ISeq(children), pivots)
-    && |pivots| + 1 == |children|
-    && 0 <= parentIdx <= PSA.psaNumStrings(parent.keys) as int
-    && 0 <= childrenIdx <= |children|
-    && (childrenIdx < |children| ==> 0 <= childIdx <= PSA.psaNumStrings(children[childrenIdx].keys) as int)
-    && |acc| == childrenIdx
-    && (forall i | 0 <= i < childrenIdx :: WF(acc[i]))
-    && ISeq(acc) == BucketListFlushPartial(I(parent), ISeq(children), pivots, childrenIdx)
-    && WF(cur)
-    && (childrenIdx < |children| ==> I(cur) == BucketListItemFlush(I(prefix(parent, parentIdx)), I(prefix(children[childrenIdx], childIdx)), pivots, childrenIdx))
-    && (childrenIdx < |children| && childIdx > 0 && parentIdx < PSA.psaNumStrings(parent.keys) as int ==> lt(PSA.psaElement(children[childrenIdx].keys, childIdx as uint64 - 1), PSA.psaElement(parent.keys, parentIdx as uint64)))
-    && (childrenIdx > 0 && childrenIdx - 1 < |pivots| && parentIdx < PSA.psaNumStrings(parent.keys) as int ==> lte(pivots[childrenIdx - 1], PSA.psaElement(parent.keys, parentIdx as uint64)))
-    && (parentIdx > 0 && childrenIdx < |children| && childIdx < PSA.psaNumStrings(children[childrenIdx].keys) as int ==> lt(PSA.psaElement(parent.keys, parentIdx as uint64 - 1), PSA.psaElement(children[childrenIdx].keys, childIdx as uint64)))
-    && (parentIdx > 0 && childrenIdx < |pivots| ==> lt(PSA.psaElement(parent.keys, parentIdx as uint64 - 1), pivots[childrenIdx]))
-  }
+  // predicate flushIterateInv(parent: Kvl, children: seq<Kvl>, pivots: seq<Key>,
+  //     parentIdx: int, childrenIdx: int, childIdx: int, acc: seq<Kvl>, cur: Kvl)
+  // {
+  //   && WF(parent)
+  //   && (forall i | 0 <= i < |children| :: WF(children[i]))
+  //   && WFBucketListProper(ISeq(children), pivots)
+  //   && |pivots| + 1 == |children|
+  //   && 0 <= parentIdx <= PSA.psaNumStrings(parent.keys) as int
+  //   && 0 <= childrenIdx <= |children|
+  //   && (childrenIdx < |children| ==> 0 <= childIdx <= PSA.psaNumStrings(children[childrenIdx].keys) as int)
+  //   && |acc| == childrenIdx
+  //   && (forall i | 0 <= i < childrenIdx :: WF(acc[i]))
+  //   && ISeq(acc) == BucketListFlushPartial(I(parent), ISeq(children), pivots, childrenIdx)
+  //   && WF(cur)
+  //   && (childrenIdx < |children| ==> I(cur) == BucketListItemFlush(I(prefix(parent, parentIdx)), I(prefix(children[childrenIdx], childIdx)), pivots, childrenIdx))
+  //   && (childrenIdx < |children| && childIdx > 0 && parentIdx < PSA.psaNumStrings(parent.keys) as int ==> lt(PSA.psaElement(children[childrenIdx].keys, childIdx as uint64 - 1), PSA.psaElement(parent.keys, parentIdx as uint64)))
+  //   && (childrenIdx > 0 && childrenIdx - 1 < |pivots| && parentIdx < PSA.psaNumStrings(parent.keys) as int ==> lte(pivots[childrenIdx - 1], PSA.psaElement(parent.keys, parentIdx as uint64)))
+  //   && (parentIdx > 0 && childrenIdx < |children| && childIdx < PSA.psaNumStrings(children[childrenIdx].keys) as int ==> lt(PSA.psaElement(parent.keys, parentIdx as uint64 - 1), PSA.psaElement(children[childrenIdx].keys, childIdx as uint64)))
+  //   && (parentIdx > 0 && childrenIdx < |pivots| ==> lt(PSA.psaElement(parent.keys, parentIdx as uint64 - 1), pivots[childrenIdx]))
+  // }
 
-  lemma flushIterateCurLastLt(parent: Kvl, children: seq<Kvl>, pivots: seq<Key>,
-      parentIdx: int, childrenIdx: int, childIdx: int, acc: seq<Kvl>, cur: Kvl)
-  requires flushIterateInv(parent, children, pivots, parentIdx, childrenIdx, childIdx, acc, cur)
-  requires childrenIdx < |children|
-  ensures PSA.psaNumStrings(cur.keys) as int > 0 && parentIdx < PSA.psaNumStrings(parent.keys) as int ==> lt(PSA.LastElement(cur.keys), PSA.psaElement(parent.keys, parentIdx as uint64))
-  ensures PSA.psaNumStrings(cur.keys) as int > 0 && childIdx < PSA.psaNumStrings(children[childrenIdx].keys) as int ==> lt(PSA.LastElement(cur.keys), PSA.psaElement(children[childrenIdx].keys, childIdx as uint64))
-  {
-    reveal_IMap();
-    if (PSA.psaNumStrings(cur.keys) as int > 0) {
-      var lastCurKey := PSA.LastElement(cur.keys);
-      assert lastCurKey in IMap(cur);
-      assert lastCurKey in (IMap(prefix(parent, parentIdx)).Keys + IMap(prefix(children[childrenIdx], childIdx)).Keys);
-      if lastCurKey in IMap(prefix(parent, parentIdx)).Keys {
-        var i := IndexOfKey(prefix(parent, parentIdx), lastCurKey);
-        assert PSA.psaElement(parent.keys, i as uint64) == lastCurKey;
-        if parentIdx < PSA.psaNumStrings(parent.keys) as int {
-          IsStrictlySortedImpliesLt(PSA.I(parent.keys), i, parentIdx);
-        }
-        if childIdx < PSA.psaNumStrings(children[childrenIdx].keys) as int {
-          IsStrictlySortedImpliesLte(PSA.I(parent.keys), i, parentIdx - 1);
-        }
-      } else {
-        var i := IndexOfKey(prefix(children[childrenIdx], childIdx), lastCurKey);
-        assert PSA.psaElement(children[childrenIdx].keys, i as uint64) == lastCurKey;
-        if parentIdx < PSA.psaNumStrings(parent.keys) as int {
-          IsStrictlySortedImpliesLte(PSA.I(children[childrenIdx].keys), i, childIdx - 1);
-        }
-        if childIdx < PSA.psaNumStrings(children[childrenIdx].keys) as int {
-          IsStrictlySortedImpliesLt(PSA.I(children[childrenIdx].keys), i, childIdx);
-        }
-      }
-    }
-  }
+  // lemma flushIterateCurLastLt(parent: Kvl, children: seq<Kvl>, pivots: seq<Key>,
+  //     parentIdx: int, childrenIdx: int, childIdx: int, acc: seq<Kvl>, cur: Kvl)
+  // requires flushIterateInv(parent, children, pivots, parentIdx, childrenIdx, childIdx, acc, cur)
+  // requires childrenIdx < |children|
+  // ensures PSA.psaNumStrings(cur.keys) as int > 0 && parentIdx < PSA.psaNumStrings(parent.keys) as int ==> lt(PSA.LastElement(cur.keys), PSA.psaElement(parent.keys, parentIdx as uint64))
+  // ensures PSA.psaNumStrings(cur.keys) as int > 0 && childIdx < PSA.psaNumStrings(children[childrenIdx].keys) as int ==> lt(PSA.LastElement(cur.keys), PSA.psaElement(children[childrenIdx].keys, childIdx as uint64))
+  // {
+  //   reveal_IMap();
+  //   if (PSA.psaNumStrings(cur.keys) as int > 0) {
+  //     var lastCurKey := PSA.LastElement(cur.keys);
+  //     assert lastCurKey in IMap(cur);
+  //     assert lastCurKey in (IMap(prefix(parent, parentIdx)).Keys + IMap(prefix(children[childrenIdx], childIdx)).Keys);
+  //     if lastCurKey in IMap(prefix(parent, parentIdx)).Keys {
+  //       var i := IndexOfKey(prefix(parent, parentIdx), lastCurKey);
+  //       assert PSA.psaElement(parent.keys, i as uint64) == lastCurKey;
+  //       if parentIdx < PSA.psaNumStrings(parent.keys) as int {
+  //         IsStrictlySortedImpliesLt(PSA.I(parent.keys), i, parentIdx);
+  //       }
+  //       if childIdx < PSA.psaNumStrings(children[childrenIdx].keys) as int {
+  //         IsStrictlySortedImpliesLte(PSA.I(parent.keys), i, parentIdx - 1);
+  //       }
+  //     } else {
+  //       var i := IndexOfKey(prefix(children[childrenIdx], childIdx), lastCurKey);
+  //       assert PSA.psaElement(children[childrenIdx].keys, i as uint64) == lastCurKey;
+  //       if parentIdx < PSA.psaNumStrings(parent.keys) as int {
+  //         IsStrictlySortedImpliesLte(PSA.I(children[childrenIdx].keys), i, childIdx - 1);
+  //       }
+  //       if childIdx < PSA.psaNumStrings(children[childrenIdx].keys) as int {
+  //         IsStrictlySortedImpliesLt(PSA.I(children[childrenIdx].keys), i, childIdx);
+  //       }
+  //     }
+  //   }
+  // }
 
-  lemma flushIterateNextsNotInPrefixes(parent: Kvl, children: seq<Kvl>, pivots: seq<Key>,
-      parentIdx: int, childrenIdx: int, childIdx: int, acc: seq<Kvl>, cur: Kvl)
-  requires flushIterateInv(parent, children, pivots, parentIdx, childrenIdx, childIdx, acc, cur)
-  requires childrenIdx < |children|
-  ensures parentIdx < PSA.psaNumStrings(parent.keys) as int ==> PSA.psaElement(parent.keys, parentIdx as uint64) !in IMap(prefix(parent, parentIdx))
-  ensures parentIdx < PSA.psaNumStrings(parent.keys) as int ==> PSA.psaElement(parent.keys, parentIdx as uint64) !in IMap(prefix(children[childrenIdx], childIdx))
-  ensures childIdx < PSA.psaNumStrings(children[childrenIdx].keys) as int ==> PSA.psaElement(children[childrenIdx].keys, childIdx as uint64) !in IMap(prefix(parent, parentIdx))
-  ensures childIdx < PSA.psaNumStrings(children[childrenIdx].keys) as int ==> PSA.psaElement(children[childrenIdx].keys, childIdx as uint64) !in IMap(prefix(children[childrenIdx], childIdx))
-  {
-    if parentIdx < PSA.psaNumStrings(parent.keys) as int && PSA.psaElement(parent.keys, parentIdx as uint64) in IMap(prefix(parent, parentIdx)) {
-      var i := IndexOfKey(prefix(parent, parentIdx), PSA.psaElement(parent.keys, parentIdx as uint64));
-      IsStrictlySortedImpliesLt(PSA.I(parent.keys), i, parentIdx);
-    }
-    if parentIdx < PSA.psaNumStrings(parent.keys) as int && PSA.psaElement(parent.keys, parentIdx as uint64) in IMap(prefix(children[childrenIdx], childIdx)) {
-      var i := IndexOfKey(prefix(children[childrenIdx], childIdx), PSA.psaElement(parent.keys, parentIdx as uint64));
-      IsStrictlySortedImpliesLte(PSA.I(children[childrenIdx].keys), i, childIdx - 1);
-    }
-    if childIdx < PSA.psaNumStrings(children[childrenIdx].keys) as int && PSA.psaElement(children[childrenIdx].keys, childIdx as uint64) in IMap(prefix(parent, parentIdx)) {
-      var i := IndexOfKey(prefix(parent, parentIdx), PSA.psaElement(children[childrenIdx].keys, childIdx as uint64));
-      IsStrictlySortedImpliesLte(PSA.I(parent.keys), i, parentIdx - 1);
-    }
-    if childIdx < PSA.psaNumStrings(children[childrenIdx].keys) as int && PSA.psaElement(children[childrenIdx].keys, childIdx as uint64) in IMap(prefix(children[childrenIdx], childIdx)) {
-      var i := IndexOfKey(prefix(children[childrenIdx], childIdx), PSA.psaElement(children[childrenIdx].keys, childIdx as uint64));
-      IsStrictlySortedImpliesLt(PSA.I(children[childrenIdx].keys), i, childIdx);
-    }
-  }
+  // lemma flushIterateNextsNotInPrefixes(parent: Kvl, children: seq<Kvl>, pivots: seq<Key>,
+  //     parentIdx: int, childrenIdx: int, childIdx: int, acc: seq<Kvl>, cur: Kvl)
+  // requires flushIterateInv(parent, children, pivots, parentIdx, childrenIdx, childIdx, acc, cur)
+  // requires childrenIdx < |children|
+  // ensures parentIdx < PSA.psaNumStrings(parent.keys) as int ==> PSA.psaElement(parent.keys, parentIdx as uint64) !in IMap(prefix(parent, parentIdx))
+  // ensures parentIdx < PSA.psaNumStrings(parent.keys) as int ==> PSA.psaElement(parent.keys, parentIdx as uint64) !in IMap(prefix(children[childrenIdx], childIdx))
+  // ensures childIdx < PSA.psaNumStrings(children[childrenIdx].keys) as int ==> PSA.psaElement(children[childrenIdx].keys, childIdx as uint64) !in IMap(prefix(parent, parentIdx))
+  // ensures childIdx < PSA.psaNumStrings(children[childrenIdx].keys) as int ==> PSA.psaElement(children[childrenIdx].keys, childIdx as uint64) !in IMap(prefix(children[childrenIdx], childIdx))
+  // {
+  //   if parentIdx < PSA.psaNumStrings(parent.keys) as int && PSA.psaElement(parent.keys, parentIdx as uint64) in IMap(prefix(parent, parentIdx)) {
+  //     var i := IndexOfKey(prefix(parent, parentIdx), PSA.psaElement(parent.keys, parentIdx as uint64));
+  //     IsStrictlySortedImpliesLt(PSA.I(parent.keys), i, parentIdx);
+  //   }
+  //   if parentIdx < PSA.psaNumStrings(parent.keys) as int && PSA.psaElement(parent.keys, parentIdx as uint64) in IMap(prefix(children[childrenIdx], childIdx)) {
+  //     var i := IndexOfKey(prefix(children[childrenIdx], childIdx), PSA.psaElement(parent.keys, parentIdx as uint64));
+  //     IsStrictlySortedImpliesLte(PSA.I(children[childrenIdx].keys), i, childIdx - 1);
+  //   }
+  //   if childIdx < PSA.psaNumStrings(children[childrenIdx].keys) as int && PSA.psaElement(children[childrenIdx].keys, childIdx as uint64) in IMap(prefix(parent, parentIdx)) {
+  //     var i := IndexOfKey(prefix(parent, parentIdx), PSA.psaElement(children[childrenIdx].keys, childIdx as uint64));
+  //     IsStrictlySortedImpliesLte(PSA.I(parent.keys), i, parentIdx - 1);
+  //   }
+  //   if childIdx < PSA.psaNumStrings(children[childrenIdx].keys) as int && PSA.psaElement(children[childrenIdx].keys, childIdx as uint64) in IMap(prefix(children[childrenIdx], childIdx)) {
+  //     var i := IndexOfKey(prefix(children[childrenIdx], childIdx), PSA.psaElement(children[childrenIdx].keys, childIdx as uint64));
+  //     IsStrictlySortedImpliesLt(PSA.I(children[childrenIdx].keys), i, childIdx);
+  //   }
+  // }
 
-  lemma flushIterateAppendParent(parent: Kvl, children: seq<Kvl>, pivots: seq<Key>,
-      parentIdx: int, childrenIdx: int, childIdx: int, acc: seq<Kvl>, cur: Kvl)
-  requires flushIterateInv(parent, children, pivots, parentIdx, childrenIdx, childIdx, acc, cur)
-  requires 0 <= childrenIdx < |children|
-  requires 0 <= parentIdx < PSA.psaNumStrings(parent.keys) as int
-  requires childrenIdx < |pivots| ==> lt(PSA.psaElement(parent.keys, parentIdx as uint64), pivots[childrenIdx])
-  ensures WF(append(cur, PSA.psaElement(parent.keys, parentIdx as uint64), parent.messages[parentIdx]))
-  ensures I(append(cur, PSA.psaElement(parent.keys, parentIdx as uint64), parent.messages[parentIdx]))
-      == BucketListItemFlush(I(prefix(parent, parentIdx + 1)), I(prefix(children[childrenIdx], childIdx)), pivots, childrenIdx)
-  {
-    flushIterateCurLastLt(parent, children, pivots, parentIdx, childrenIdx, childIdx, acc, cur);
-    flushIterateNextsNotInPrefixes(parent, children, pivots, parentIdx, childrenIdx, childIdx, acc, cur);
-    StrictlySortedAugment(PSA.I(cur.keys), PSA.psaElement(parent.keys, parentIdx as uint64));
-    BucketListItemFlushAddParentKey(I(prefix(parent, parentIdx)), I(prefix(children[childrenIdx], childIdx)), pivots, PSA.psaElement(parent.keys, parentIdx as uint64), parent.messages[parentIdx]);
+  // lemma flushIterateAppendParent(parent: Kvl, children: seq<Kvl>, pivots: seq<Key>,
+  //     parentIdx: int, childrenIdx: int, childIdx: int, acc: seq<Kvl>, cur: Kvl)
+  // requires flushIterateInv(parent, children, pivots, parentIdx, childrenIdx, childIdx, acc, cur)
+  // requires 0 <= childrenIdx < |children|
+  // requires 0 <= parentIdx < PSA.psaNumStrings(parent.keys) as int
+  // requires childrenIdx < |pivots| ==> lt(PSA.psaElement(parent.keys, parentIdx as uint64), pivots[childrenIdx])
+  // ensures WF(append(cur, PSA.psaElement(parent.keys, parentIdx as uint64), parent.messages[parentIdx]))
+  // ensures I(append(cur, PSA.psaElement(parent.keys, parentIdx as uint64), parent.messages[parentIdx]))
+  //     == BucketListItemFlush(I(prefix(parent, parentIdx + 1)), I(prefix(children[childrenIdx], childIdx)), pivots, childrenIdx)
+  // {
+  //   flushIterateCurLastLt(parent, children, pivots, parentIdx, childrenIdx, childIdx, acc, cur);
+  //   flushIterateNextsNotInPrefixes(parent, children, pivots, parentIdx, childrenIdx, childIdx, acc, cur);
+  //   StrictlySortedAugment(PSA.I(cur.keys), PSA.psaElement(parent.keys, parentIdx as uint64));
+  //   BucketListItemFlushAddParentKey(I(prefix(parent, parentIdx)), I(prefix(children[childrenIdx], childIdx)), pivots, PSA.psaElement(parent.keys, parentIdx as uint64), parent.messages[parentIdx]);
 
-    P.RouteIs(pivots, PSA.psaElement(parent.keys, parentIdx as uint64), childrenIdx);
+  //   P.RouteIs(pivots, PSA.psaElement(parent.keys, parentIdx as uint64), childrenIdx);
 
-    Iappend(cur, PSA.psaElement(parent.keys, parentIdx as uint64), parent.messages[parentIdx]);
-    Iprefix_append(parent, parentIdx);
+  //   Iappend(cur, PSA.psaElement(parent.keys, parentIdx as uint64), parent.messages[parentIdx]);
+  //   Iprefix_append(parent, parentIdx);
 
-    /*assert I(append(cur, PSA.psaElement(parent.keys, parentIdx as uint64), parent.messages[parentIdx]))
-        == I(cur)[PSA.psaElement(parent.keys, parentIdx as uint64) := parent.messages[parentIdx]]
-        == BucketListItemFlush(I(prefix(parent, parentIdx)), I(prefix(children[childrenIdx], childIdx)), pivots, childrenIdx)[PSA.psaElement(parent.keys, parentIdx as uint64) := parent.messages[parentIdx]]
-        == BucketListItemFlush(I(prefix(parent, parentIdx))[PSA.psaElement(parent.keys, parentIdx as uint64) := parent.messages[parentIdx]], I(prefix(children[childrenIdx], childIdx)), pivots, childrenIdx)
-        == BucketListItemFlush(I(prefix(parent, parentIdx + 1)), I(prefix(children[childrenIdx], childIdx)), pivots, childrenIdx);*/
-  }
+  //   /*assert I(append(cur, PSA.psaElement(parent.keys, parentIdx as uint64), parent.messages[parentIdx]))
+  //       == I(cur)[PSA.psaElement(parent.keys, parentIdx as uint64) := parent.messages[parentIdx]]
+  //       == BucketListItemFlush(I(prefix(parent, parentIdx)), I(prefix(children[childrenIdx], childIdx)), pivots, childrenIdx)[PSA.psaElement(parent.keys, parentIdx as uint64) := parent.messages[parentIdx]]
+  //       == BucketListItemFlush(I(prefix(parent, parentIdx))[PSA.psaElement(parent.keys, parentIdx as uint64) := parent.messages[parentIdx]], I(prefix(children[childrenIdx], childIdx)), pivots, childrenIdx)
+  //       == BucketListItemFlush(I(prefix(parent, parentIdx + 1)), I(prefix(children[childrenIdx], childIdx)), pivots, childrenIdx);*/
+  // }
 
-  lemma flushIterateAppendChild(parent: Kvl, children: seq<Kvl>, pivots: seq<Key>,
-      parentIdx: int, childrenIdx: int, childIdx: int, acc: seq<Kvl>, cur: Kvl)
-  requires flushIterateInv(parent, children, pivots, parentIdx, childrenIdx, childIdx, acc, cur)
-  requires 0 <= childrenIdx < |children|
-  requires 0 <= childIdx < PSA.psaNumStrings(children[childrenIdx].keys) as int
-  ensures WF(append(cur, PSA.psaElement(children[childrenIdx].keys, childIdx as uint64), children[childrenIdx].messages[childIdx]))
-  ensures I(append(cur, PSA.psaElement(children[childrenIdx].keys, childIdx as uint64), children[childrenIdx].messages[childIdx]))
-      == BucketListItemFlush(I(prefix(parent, parentIdx)), I(prefix(children[childrenIdx], childIdx + 1)), pivots, childrenIdx)
-  {
-    var child := children[childrenIdx];
-    flushIterateCurLastLt(parent, children, pivots, parentIdx, childrenIdx, childIdx, acc, cur);
-    flushIterateNextsNotInPrefixes(parent, children, pivots, parentIdx, childrenIdx, childIdx, acc, cur);
-    StrictlySortedAugment(PSA.I(cur.keys), PSA.psaElement(child.keys, childIdx as uint64));
-    BucketListItemFlushAddChildKey(I(prefix(parent, parentIdx)), I(prefix(children[childrenIdx], childIdx)), pivots, PSA.psaElement(child.keys, childIdx as uint64), child.messages[childIdx]);
+  // lemma flushIterateAppendChild(parent: Kvl, children: seq<Kvl>, pivots: seq<Key>,
+  //     parentIdx: int, childrenIdx: int, childIdx: int, acc: seq<Kvl>, cur: Kvl)
+  // requires flushIterateInv(parent, children, pivots, parentIdx, childrenIdx, childIdx, acc, cur)
+  // requires 0 <= childrenIdx < |children|
+  // requires 0 <= childIdx < PSA.psaNumStrings(children[childrenIdx].keys) as int
+  // ensures WF(append(cur, PSA.psaElement(children[childrenIdx].keys, childIdx as uint64), children[childrenIdx].messages[childIdx]))
+  // ensures I(append(cur, PSA.psaElement(children[childrenIdx].keys, childIdx as uint64), children[childrenIdx].messages[childIdx]))
+  //     == BucketListItemFlush(I(prefix(parent, parentIdx)), I(prefix(children[childrenIdx], childIdx + 1)), pivots, childrenIdx)
+  // {
+  //   var child := children[childrenIdx];
+  //   flushIterateCurLastLt(parent, children, pivots, parentIdx, childrenIdx, childIdx, acc, cur);
+  //   flushIterateNextsNotInPrefixes(parent, children, pivots, parentIdx, childrenIdx, childIdx, acc, cur);
+  //   StrictlySortedAugment(PSA.I(cur.keys), PSA.psaElement(child.keys, childIdx as uint64));
+  //   BucketListItemFlushAddChildKey(I(prefix(parent, parentIdx)), I(prefix(children[childrenIdx], childIdx)), pivots, PSA.psaElement(child.keys, childIdx as uint64), child.messages[childIdx]);
 
-    assert WFBucketAt(I(children[childrenIdx]), pivots, childrenIdx);
-    Imaps(child, childIdx);
-    assert PSA.psaElement(child.keys, childIdx as uint64) in IMap(children[childrenIdx]);
-    assert P.Route(pivots, PSA.psaElement(child.keys, childIdx as uint64)) == childrenIdx;
+  //   assert WFBucketAt(I(children[childrenIdx]), pivots, childrenIdx);
+  //   Imaps(child, childIdx);
+  //   assert PSA.psaElement(child.keys, childIdx as uint64) in IMap(children[childrenIdx]);
+  //   assert P.Route(pivots, PSA.psaElement(child.keys, childIdx as uint64)) == childrenIdx;
 
-    Iappend(cur, PSA.psaElement(child.keys, childIdx as uint64), child.messages[childIdx]);
-    Iprefix_append(child, childIdx);
+  //   Iappend(cur, PSA.psaElement(child.keys, childIdx as uint64), child.messages[childIdx]);
+  //   Iprefix_append(child, childIdx);
 
-    /*assert I(append(cur, PSA.psaElement(child.keys, childIdx as uint64), child.messages[childIdx]))
-        == I(cur)[PSA.psaElement(child.keys, childIdx as uint64) := child.messages[childIdx]]
-        == BucketListItemFlush(I(prefix(parent, parentIdx)), I(prefix(children[childrenIdx], childIdx)), pivots, childrenIdx)[PSA.psaElement(child.keys, childIdx as uint64) := child.messages[childIdx]]
-        == BucketListItemFlush(I(prefix(parent, parentIdx)), I(prefix(children[childrenIdx], childIdx))[PSA.psaElement(child.keys, childIdx as uint64) := child.messages[childIdx]], pivots, childrenIdx)
-        == BucketListItemFlush(I(prefix(parent, parentIdx)), I(prefix(children[childrenIdx], childIdx + 1)), pivots, childrenIdx);*/
-  }
+  //   /*assert I(append(cur, PSA.psaElement(child.keys, childIdx as uint64), child.messages[childIdx]))
+  //       == I(cur)[PSA.psaElement(child.keys, childIdx as uint64) := child.messages[childIdx]]
+  //       == BucketListItemFlush(I(prefix(parent, parentIdx)), I(prefix(children[childrenIdx], childIdx)), pivots, childrenIdx)[PSA.psaElement(child.keys, childIdx as uint64) := child.messages[childIdx]]
+  //       == BucketListItemFlush(I(prefix(parent, parentIdx)), I(prefix(children[childrenIdx], childIdx))[PSA.psaElement(child.keys, childIdx as uint64) := child.messages[childIdx]], pivots, childrenIdx)
+  //       == BucketListItemFlush(I(prefix(parent, parentIdx)), I(prefix(children[childrenIdx], childIdx + 1)), pivots, childrenIdx);*/
+  // }
 
-  lemma {:fuel BucketListItemFlush,0} {:fuel P.Route,0}
-  flushIterateAppendParentAndChild(parent: Kvl, children: seq<Kvl>, pivots: seq<Key>,
-      parentIdx: int, childrenIdx: int, childIdx: int, acc: seq<Kvl>, cur: Kvl)
-  requires flushIterateInv(parent, children, pivots, parentIdx, childrenIdx, childIdx, acc, cur)
-  requires 0 <= childrenIdx < |children|
-  requires 0 <= parentIdx < PSA.psaNumStrings(parent.keys) as int
-  requires 0 <= childIdx < PSA.psaNumStrings(children[childrenIdx].keys) as int
-  requires PSA.psaElement(children[childrenIdx].keys, childIdx as uint64) == PSA.psaElement(parent.keys, parentIdx as uint64)
-  requires Merge(parent.messages[parentIdx], children[childrenIdx].messages[childIdx]) != IdentityMessage()
+  // lemma {:fuel BucketListItemFlush,0} {:fuel P.Route,0}
+  // flushIterateAppendParentAndChild(parent: Kvl, children: seq<Kvl>, pivots: seq<Key>,
+  //     parentIdx: int, childrenIdx: int, childIdx: int, acc: seq<Kvl>, cur: Kvl)
+  // requires flushIterateInv(parent, children, pivots, parentIdx, childrenIdx, childIdx, acc, cur)
+  // requires 0 <= childrenIdx < |children|
+  // requires 0 <= parentIdx < PSA.psaNumStrings(parent.keys) as int
+  // requires 0 <= childIdx < PSA.psaNumStrings(children[childrenIdx].keys) as int
+  // requires PSA.psaElement(children[childrenIdx].keys, childIdx as uint64) == PSA.psaElement(parent.keys, parentIdx as uint64)
+  // requires Merge(parent.messages[parentIdx], children[childrenIdx].messages[childIdx]) != IdentityMessage()
 
-  ensures WF(append(cur, PSA.psaElement(parent.keys, parentIdx as uint64), Merge(parent.messages[parentIdx], children[childrenIdx].messages[childIdx])))
-  ensures I(append(cur, PSA.psaElement(parent.keys, parentIdx as uint64), Merge(parent.messages[parentIdx], children[childrenIdx].messages[childIdx])))
-      == BucketListItemFlush(I(prefix(parent, parentIdx + 1)), I(prefix(children[childrenIdx], childIdx + 1)), pivots, childrenIdx)
-  {
-    var child := children[childrenIdx];
-    flushIterateCurLastLt(parent, children, pivots, parentIdx, childrenIdx, childIdx, acc, cur);
-    flushIterateNextsNotInPrefixes(parent, children, pivots, parentIdx, childrenIdx, childIdx, acc, cur);
-    StrictlySortedAugment(PSA.I(cur.keys), PSA.psaElement(child.keys, childIdx as uint64));
-    BucketListItemFlushAddParentAndChildKey(I(prefix(parent, parentIdx)), I(prefix(children[childrenIdx], childIdx)), pivots, PSA.psaElement(child.keys, childIdx as uint64), parent.messages[parentIdx], child.messages[childIdx]);
+  // ensures WF(append(cur, PSA.psaElement(parent.keys, parentIdx as uint64), Merge(parent.messages[parentIdx], children[childrenIdx].messages[childIdx])))
+  // ensures I(append(cur, PSA.psaElement(parent.keys, parentIdx as uint64), Merge(parent.messages[parentIdx], children[childrenIdx].messages[childIdx])))
+  //     == BucketListItemFlush(I(prefix(parent, parentIdx + 1)), I(prefix(children[childrenIdx], childIdx + 1)), pivots, childrenIdx)
+  // {
+  //   var child := children[childrenIdx];
+  //   flushIterateCurLastLt(parent, children, pivots, parentIdx, childrenIdx, childIdx, acc, cur);
+  //   flushIterateNextsNotInPrefixes(parent, children, pivots, parentIdx, childrenIdx, childIdx, acc, cur);
+  //   StrictlySortedAugment(PSA.I(cur.keys), PSA.psaElement(child.keys, childIdx as uint64));
+  //   BucketListItemFlushAddParentAndChildKey(I(prefix(parent, parentIdx)), I(prefix(children[childrenIdx], childIdx)), pivots, PSA.psaElement(child.keys, childIdx as uint64), parent.messages[parentIdx], child.messages[childIdx]);
 
-    assert WFBucketAt(I(children[childrenIdx]), pivots, childrenIdx);
-    Imaps(child, childIdx);
-    assert PSA.psaElement(child.keys, childIdx as uint64) in IMap(children[childrenIdx]);
-    assert P.Route(pivots, PSA.psaElement(child.keys, childIdx as uint64)) == childrenIdx;
+  //   assert WFBucketAt(I(children[childrenIdx]), pivots, childrenIdx);
+  //   Imaps(child, childIdx);
+  //   assert PSA.psaElement(child.keys, childIdx as uint64) in IMap(children[childrenIdx]);
+  //   assert P.Route(pivots, PSA.psaElement(child.keys, childIdx as uint64)) == childrenIdx;
 
-    Iappend(cur, PSA.psaElement(parent.keys, parentIdx as uint64), Merge(parent.messages[parentIdx], children[childrenIdx].messages[childIdx]));
-    Iprefix_append(parent, parentIdx);
-    Iprefix_append(child, childIdx);
+  //   Iappend(cur, PSA.psaElement(parent.keys, parentIdx as uint64), Merge(parent.messages[parentIdx], children[childrenIdx].messages[childIdx]));
+  //   Iprefix_append(parent, parentIdx);
+  //   Iprefix_append(child, childIdx);
 
-    /*assert I(append(cur, PSA.psaElement(parent.keys, parentIdx as uint64), Merge(parent.messages[parentIdx], children[childrenIdx].messages[childIdx])))
-        == I(cur)[PSA.psaElement(parent.keys, parentIdx as uint64) := Merge(parent.messages[parentIdx], children[childrenIdx].messages[childIdx])]
-        == BucketListItemFlush(I(prefix(parent, parentIdx)), I(prefix(children[childrenIdx], childIdx)), pivots, childrenIdx)[PSA.psaElement(parent.keys, parentIdx as uint64) := Merge(parent.messages[parentIdx], children[childrenIdx].messages[childIdx])]
-        == BucketListItemFlush(I(prefix(parent, parentIdx))[PSA.psaElement(parent.keys, parentIdx as uint64) := parent.messages[parentIdx]], I(prefix(children[childrenIdx], childIdx))[PSA.psaElement(child.keys, childIdx as uint64) := child.messages[childIdx]], pivots, childrenIdx)
-        == BucketListItemFlush(I(prefix(parent, parentIdx + 1)), I(prefix(children[childrenIdx], childIdx + 1)), pivots, childrenIdx);*/
-  }
+  //   /*assert I(append(cur, PSA.psaElement(parent.keys, parentIdx as uint64), Merge(parent.messages[parentIdx], children[childrenIdx].messages[childIdx])))
+  //       == I(cur)[PSA.psaElement(parent.keys, parentIdx as uint64) := Merge(parent.messages[parentIdx], children[childrenIdx].messages[childIdx])]
+  //       == BucketListItemFlush(I(prefix(parent, parentIdx)), I(prefix(children[childrenIdx], childIdx)), pivots, childrenIdx)[PSA.psaElement(parent.keys, parentIdx as uint64) := Merge(parent.messages[parentIdx], children[childrenIdx].messages[childIdx])]
+  //       == BucketListItemFlush(I(prefix(parent, parentIdx))[PSA.psaElement(parent.keys, parentIdx as uint64) := parent.messages[parentIdx]], I(prefix(children[childrenIdx], childIdx))[PSA.psaElement(child.keys, childIdx as uint64) := child.messages[childIdx]], pivots, childrenIdx)
+  //       == BucketListItemFlush(I(prefix(parent, parentIdx + 1)), I(prefix(children[childrenIdx], childIdx + 1)), pivots, childrenIdx);*/
+  // }
 
-  lemma flushIterateCurEqBucketListItemFlush(parent: Kvl, children: seq<Kvl>, pivots: seq<Key>,
-      parentIdx: int, childrenIdx: int, childIdx: int, acc: seq<Kvl>, cur: Kvl)
-  requires flushIterateInv(parent, children, pivots, parentIdx, childrenIdx, childIdx, acc, cur)
-  requires childrenIdx < |children|
-  requires childIdx == PSA.psaNumStrings(children[childrenIdx].keys) as int
-  requires parentIdx < PSA.psaNumStrings(parent.keys) as int ==> childrenIdx < |pivots| && lte(pivots[childrenIdx], PSA.psaElement(parent.keys, parentIdx as uint64))
-  ensures I(cur) == BucketListItemFlush(I(parent), I(children[childrenIdx]), pivots, childrenIdx)
-  {
-    forall key | P.Route(pivots, key) == childrenIdx
-    ensures MapsAgreeOnKey(IMap(prefix(parent, parentIdx)), IMap(parent), key)
-    {
-      WFPrefix(parent, parentIdx);
-      if (key in IMap(prefix(parent, parentIdx))) {
-        var i := IndexOfKey(prefix(parent, parentIdx), key);
-        Imaps(parent, i);
-        Imaps(prefix(parent, parentIdx), i);
-      } else if (key in IMap(parent)) {
-        var i := IndexOfKey(parent, key);
-        if (i < parentIdx) {
-          Imaps(parent, i);
-          Imaps(prefix(parent, parentIdx), i);
-        } else {
-          assert lt(PSA.psaElement(parent.keys, i as uint64), pivots[childrenIdx]);
-          assert lte(pivots[childrenIdx], PSA.psaElement(parent.keys, parentIdx as uint64));
-          IsStrictlySortedImpliesLte(PSA.I(parent.keys), parentIdx, i);
-          assert false;
-        }
-      }
-    }
-    BucketListItemFlushEq(I(prefix(parent, parentIdx)), I(parent), I(prefix(children[childrenIdx], childIdx)), pivots, childrenIdx);
-    assert prefix(children[childrenIdx], childIdx) == children[childrenIdx];
-  }
+  // lemma flushIterateCurEqBucketListItemFlush(parent: Kvl, children: seq<Kvl>, pivots: seq<Key>,
+  //     parentIdx: int, childrenIdx: int, childIdx: int, acc: seq<Kvl>, cur: Kvl)
+  // requires flushIterateInv(parent, children, pivots, parentIdx, childrenIdx, childIdx, acc, cur)
+  // requires childrenIdx < |children|
+  // requires childIdx == PSA.psaNumStrings(children[childrenIdx].keys) as int
+  // requires parentIdx < PSA.psaNumStrings(parent.keys) as int ==> childrenIdx < |pivots| && lte(pivots[childrenIdx], PSA.psaElement(parent.keys, parentIdx as uint64))
+  // ensures I(cur) == BucketListItemFlush(I(parent), I(children[childrenIdx]), pivots, childrenIdx)
+  // {
+  //   forall key | P.Route(pivots, key) == childrenIdx
+  //   ensures MapsAgreeOnKey(IMap(prefix(parent, parentIdx)), IMap(parent), key)
+  //   {
+  //     WFPrefix(parent, parentIdx);
+  //     if (key in IMap(prefix(parent, parentIdx))) {
+  //       var i := IndexOfKey(prefix(parent, parentIdx), key);
+  //       Imaps(parent, i);
+  //       Imaps(prefix(parent, parentIdx), i);
+  //     } else if (key in IMap(parent)) {
+  //       var i := IndexOfKey(parent, key);
+  //       if (i < parentIdx) {
+  //         Imaps(parent, i);
+  //         Imaps(prefix(parent, parentIdx), i);
+  //       } else {
+  //         assert lt(PSA.psaElement(parent.keys, i as uint64), pivots[childrenIdx]);
+  //         assert lte(pivots[childrenIdx], PSA.psaElement(parent.keys, parentIdx as uint64));
+  //         IsStrictlySortedImpliesLte(PSA.I(parent.keys), parentIdx, i);
+  //         assert false;
+  //       }
+  //     }
+  //   }
+  //   BucketListItemFlushEq(I(prefix(parent, parentIdx)), I(parent), I(prefix(children[childrenIdx], childIdx)), pivots, childrenIdx);
+  //   assert prefix(children[childrenIdx], childIdx) == children[childrenIdx];
+  // }
 
-  lemma flushIteratepivotLteChildKey0(parent: Kvl, children: seq<Kvl>, pivots: seq<Key>,
-      parentIdx: int, childrenIdx: int, childIdx: int, acc: seq<Kvl>, cur: Kvl)
-  requires flushIterateInv(parent, children, pivots, parentIdx, childrenIdx, childIdx, acc, cur)
-  ensures childrenIdx < |pivots| && PSA.psaNumStrings(children[childrenIdx + 1].keys) as int > 0 ==> lte(pivots[childrenIdx], PSA.FirstElement(children[childrenIdx + 1].keys))
-  {
-    if childrenIdx < |pivots| && PSA.psaNumStrings(children[childrenIdx + 1].keys) as int > 0 {
-      Imaps(children[childrenIdx + 1], 0);
-      assert P.Route(pivots, PSA.FirstElement(children[childrenIdx + 1].keys)) == childrenIdx + 1;
-    }
-  }
+  // lemma flushIteratepivotLteChildKey0(parent: Kvl, children: seq<Kvl>, pivots: seq<Key>,
+  //     parentIdx: int, childrenIdx: int, childIdx: int, acc: seq<Kvl>, cur: Kvl)
+  // requires flushIterateInv(parent, children, pivots, parentIdx, childrenIdx, childIdx, acc, cur)
+  // ensures childrenIdx < |pivots| && PSA.psaNumStrings(children[childrenIdx + 1].keys) as int > 0 ==> lte(pivots[childrenIdx], PSA.FirstElement(children[childrenIdx + 1].keys))
+  // {
+  //   if childrenIdx < |pivots| && PSA.psaNumStrings(children[childrenIdx + 1].keys) as int > 0 {
+  //     Imaps(children[childrenIdx + 1], 0);
+  //     assert P.Route(pivots, PSA.FirstElement(children[childrenIdx + 1].keys)) == childrenIdx + 1;
+  //   }
+  // }
 
-  lemma flushIterateIEmptyEqBucketListItemFlush(parent: Kvl, children: seq<Kvl>, pivots: seq<Key>,
-      parentIdx: int, childrenIdx: int, childIdx: int, acc: seq<Kvl>, cur: Kvl)
-  requires flushIterateInv(parent, children, pivots, parentIdx, childrenIdx, childIdx, acc, cur)
-  requires childrenIdx + 1 < |children| && parentIdx > 0 ==> lt(PSA.psaElement(parent.keys, parentIdx as uint64 - 1), pivots[childrenIdx])
-  ensures childrenIdx + 1 < |children| ==>
-         I(Kvl(PSA.EmptyPsa(),[])).b
-      == BucketListItemFlush(I(prefix(parent, parentIdx)), I(prefix(children[childrenIdx + 1], 0)), pivots, childrenIdx + 1).b
-  {
-    reveal_IMap();
-    forall key | key in IMap(prefix(parent, parentIdx))
-    ensures P.Route(pivots, key) != childrenIdx + 1
-    {
-      var i := IndexOfKey(prefix(parent, parentIdx), key);
-      IsStrictlySortedImpliesLte(PSA.I(parent.keys), i, parentIdx - 1);
-    }
-  }
+  // lemma flushIterateIEmptyEqBucketListItemFlush(parent: Kvl, children: seq<Kvl>, pivots: seq<Key>,
+  //     parentIdx: int, childrenIdx: int, childIdx: int, acc: seq<Kvl>, cur: Kvl)
+  // requires flushIterateInv(parent, children, pivots, parentIdx, childrenIdx, childIdx, acc, cur)
+  // requires childrenIdx + 1 < |children| && parentIdx > 0 ==> lt(PSA.psaElement(parent.keys, parentIdx as uint64 - 1), pivots[childrenIdx])
+  // ensures childrenIdx + 1 < |children| ==>
+  //        I(Kvl(PSA.EmptyPsa(),[])).b
+  //     == BucketListItemFlush(I(prefix(parent, parentIdx)), I(prefix(children[childrenIdx + 1], 0)), pivots, childrenIdx + 1).b
+  // {
+  //   reveal_IMap();
+  //   forall key | key in IMap(prefix(parent, parentIdx))
+  //   ensures P.Route(pivots, key) != childrenIdx + 1
+  //   {
+  //     var i := IndexOfKey(prefix(parent, parentIdx), key);
+  //     IsStrictlySortedImpliesLte(PSA.I(parent.keys), i, parentIdx - 1);
+  //   }
+  // }
 
-  lemma flushIterateRes(parent: Kvl, children: seq<Kvl>, pivots: seq<Key>,
-      parentIdx: int, childrenIdx: int, childIdx: int, acc: seq<Kvl>, cur: Kvl)
-  requires flushIterateInv(parent, children, pivots, parentIdx, childrenIdx, childIdx, acc, cur)
-  ensures var f := flushIterate(parent, children, pivots, parentIdx, childrenIdx, childIdx, acc, cur);
-      && (forall i | 0 <= i < |f| :: WF(f[i]))
-      && ISeq(f) == BucketListFlush(I(parent), ISeq(children), pivots)
-  decreases |children| - childrenIdx
-  decreases PSA.psaNumStrings(parent.keys) as int - parentIdx +
-      (if childrenIdx < |children| then PSA.psaNumStrings(children[childrenIdx].keys) as int - childIdx else 0)
-  {
-    if childrenIdx == |children| {
-    } else {
-      var child := children[childrenIdx];
+  // lemma flushIterateRes(parent: Kvl, children: seq<Kvl>, pivots: seq<Key>,
+  //     parentIdx: int, childrenIdx: int, childIdx: int, acc: seq<Kvl>, cur: Kvl)
+  // requires flushIterateInv(parent, children, pivots, parentIdx, childrenIdx, childIdx, acc, cur)
+  // ensures var f := flushIterate(parent, children, pivots, parentIdx, childrenIdx, childIdx, acc, cur);
+  //     && (forall i | 0 <= i < |f| :: WF(f[i]))
+  //     && ISeq(f) == BucketListFlush(I(parent), ISeq(children), pivots)
+  // decreases |children| - childrenIdx
+  // decreases PSA.psaNumStrings(parent.keys) as int - parentIdx +
+  //     (if childrenIdx < |children| then PSA.psaNumStrings(children[childrenIdx].keys) as int - childIdx else 0)
+  // {
+  //   if childrenIdx == |children| {
+  //   } else {
+  //     var child := children[childrenIdx];
 
-      if parentIdx + 1 < PSA.psaNumStrings(parent.keys) as int {
-        IsStrictlySortedImpliesLt(PSA.I(parent.keys), parentIdx, parentIdx + 1);
-      }
-      if childrenIdx + 1 < |pivots| {
-        IsStrictlySortedImpliesLt(pivots, childrenIdx, childrenIdx + 1);
-      }
-      if childIdx + 1 < PSA.psaNumStrings(child.keys) as int {
-        IsStrictlySortedImpliesLt(PSA.I(child.keys), childIdx, childIdx + 1);
-      }
-      if childIdx < PSA.psaNumStrings(child.keys) as int {
-        Imaps(child, childIdx);
-        assert P.Route(pivots, PSA.psaElement(child.keys, childIdx as uint64)) == childrenIdx;
-      }
+  //     if parentIdx + 1 < PSA.psaNumStrings(parent.keys) as int {
+  //       IsStrictlySortedImpliesLt(PSA.I(parent.keys), parentIdx, parentIdx + 1);
+  //     }
+  //     if childrenIdx + 1 < |pivots| {
+  //       IsStrictlySortedImpliesLt(pivots, childrenIdx, childrenIdx + 1);
+  //     }
+  //     if childIdx + 1 < PSA.psaNumStrings(child.keys) as int {
+  //       IsStrictlySortedImpliesLt(PSA.I(child.keys), childIdx, childIdx + 1);
+  //     }
+  //     if childIdx < PSA.psaNumStrings(child.keys) as int {
+  //       Imaps(child, childIdx);
+  //       assert P.Route(pivots, PSA.psaElement(child.keys, childIdx as uint64)) == childrenIdx;
+  //     }
 
-      if parentIdx == PSA.psaNumStrings(parent.keys) as int {
-        if childIdx == PSA.psaNumStrings(child.keys) as int {
-          flushIterateCurEqBucketListItemFlush(parent, children, pivots, parentIdx, childrenIdx, childIdx, acc, cur);
-          flushIterateIEmptyEqBucketListItemFlush(parent, children, pivots, parentIdx, childrenIdx, childIdx, acc, cur);
-          flushIteratepivotLteChildKey0(parent, children, pivots, parentIdx, childrenIdx, childIdx, acc, cur);
-          flushIterateRes(parent, children, pivots, parentIdx, childrenIdx + 1, 0, acc + [cur], Kvl(PSA.EmptyPsa(), []));
-        //} else if |cur| == 0 {
-        //  flushIterateRes(parent, children, pivots, parentIdx, childrenIdx + 1, 0, acc + [child], Kvl(PSA.EmptyPsa(), []));
-        } else {
-          flushIterateAppendChild(parent, children, pivots, parentIdx, childrenIdx, childIdx, acc, cur);
-          flushIterateRes(parent, children, pivots, parentIdx, childrenIdx, childIdx + 1, acc, append(cur, PSA.psaElement(child.keys, childIdx as uint64), child.messages[childIdx]));
-        }
-      } else {
-        if childIdx == PSA.psaNumStrings(child.keys) as int {
-          if childrenIdx == |children| - 1 {
-            flushIterateAppendParent(parent, children, pivots, parentIdx, childrenIdx, childIdx, acc, cur);
-            flushIterateRes(parent, children, pivots, parentIdx + 1, childrenIdx, childIdx, acc, append(cur, PSA.psaElement(parent.keys, parentIdx as uint64), parent.messages[parentIdx]));
-          } else {
-            if lt(PSA.psaElement(parent.keys, parentIdx as uint64), pivots[childrenIdx]) {
-              flushIterateAppendParent(parent, children, pivots, parentIdx, childrenIdx, childIdx, acc, cur);
-              flushIterateRes(parent, children, pivots, parentIdx + 1, childrenIdx, childIdx, acc, append(cur, PSA.psaElement(parent.keys, parentIdx as uint64), parent.messages[parentIdx]));
-            } else {
-              flushIterateCurEqBucketListItemFlush(parent, children, pivots, parentIdx, childrenIdx, childIdx, acc, cur);
-              flushIterateIEmptyEqBucketListItemFlush(parent, children, pivots, parentIdx, childrenIdx, childIdx, acc, cur);
-              flushIteratepivotLteChildKey0(parent, children, pivots, parentIdx, childrenIdx, childIdx, acc, cur);
-              flushIterateRes(parent, children, pivots, parentIdx, childrenIdx + 1, 0, acc + [cur], Kvl(PSA.EmptyPsa(), []));
-            }
-          }
-        } else {
-          if PSA.psaElement(child.keys, childIdx as uint64) == PSA.psaElement(parent.keys, parentIdx as uint64) {
-            var m := Merge(parent.messages[parentIdx], child.messages[childIdx]);
-            if m == IdentityMessage() {
-              flushIterateRes(parent, children, pivots, parentIdx + 1, childrenIdx, childIdx + 1, acc, cur);
-            } else {
-              flushIterateAppendParentAndChild(parent, children, pivots, parentIdx, childrenIdx, childIdx, acc, cur);
-              flushIterateRes(parent, children, pivots, parentIdx + 1, childrenIdx, childIdx + 1, acc, append(cur, PSA.psaElement(child.keys, childIdx as uint64), m));
-            }
-          } else if lt(PSA.psaElement(child.keys, childIdx as uint64), PSA.psaElement(parent.keys, parentIdx as uint64)) {
-            flushIterateAppendChild(parent, children, pivots, parentIdx, childrenIdx, childIdx, acc, cur);
-            flushIterateRes(parent, children, pivots, parentIdx, childrenIdx, childIdx + 1, acc, append(cur, PSA.psaElement(child.keys, childIdx as uint64), child.messages[childIdx]));
-          } else {
-            flushIterateAppendParent(parent, children, pivots, parentIdx, childrenIdx, childIdx, acc, cur);
-            flushIterateRes(parent, children, pivots, parentIdx + 1, childrenIdx, childIdx, acc, append(cur, PSA.psaElement(parent.keys, parentIdx as uint64), parent.messages[parentIdx]));
-          }
-        }
-      }
-    }
-  }
+  //     if parentIdx == PSA.psaNumStrings(parent.keys) as int {
+  //       if childIdx == PSA.psaNumStrings(child.keys) as int {
+  //         flushIterateCurEqBucketListItemFlush(parent, children, pivots, parentIdx, childrenIdx, childIdx, acc, cur);
+  //         flushIterateIEmptyEqBucketListItemFlush(parent, children, pivots, parentIdx, childrenIdx, childIdx, acc, cur);
+  //         flushIteratepivotLteChildKey0(parent, children, pivots, parentIdx, childrenIdx, childIdx, acc, cur);
+  //         flushIterateRes(parent, children, pivots, parentIdx, childrenIdx + 1, 0, acc + [cur], Kvl(PSA.EmptyPsa(), []));
+  //       //} else if |cur| == 0 {
+  //       //  flushIterateRes(parent, children, pivots, parentIdx, childrenIdx + 1, 0, acc + [child], Kvl(PSA.EmptyPsa(), []));
+  //       } else {
+  //         flushIterateAppendChild(parent, children, pivots, parentIdx, childrenIdx, childIdx, acc, cur);
+  //         flushIterateRes(parent, children, pivots, parentIdx, childrenIdx, childIdx + 1, acc, append(cur, PSA.psaElement(child.keys, childIdx as uint64), child.messages[childIdx]));
+  //       }
+  //     } else {
+  //       if childIdx == PSA.psaNumStrings(child.keys) as int {
+  //         if childrenIdx == |children| - 1 {
+  //           flushIterateAppendParent(parent, children, pivots, parentIdx, childrenIdx, childIdx, acc, cur);
+  //           flushIterateRes(parent, children, pivots, parentIdx + 1, childrenIdx, childIdx, acc, append(cur, PSA.psaElement(parent.keys, parentIdx as uint64), parent.messages[parentIdx]));
+  //         } else {
+  //           if lt(PSA.psaElement(parent.keys, parentIdx as uint64), pivots[childrenIdx]) {
+  //             flushIterateAppendParent(parent, children, pivots, parentIdx, childrenIdx, childIdx, acc, cur);
+  //             flushIterateRes(parent, children, pivots, parentIdx + 1, childrenIdx, childIdx, acc, append(cur, PSA.psaElement(parent.keys, parentIdx as uint64), parent.messages[parentIdx]));
+  //           } else {
+  //             flushIterateCurEqBucketListItemFlush(parent, children, pivots, parentIdx, childrenIdx, childIdx, acc, cur);
+  //             flushIterateIEmptyEqBucketListItemFlush(parent, children, pivots, parentIdx, childrenIdx, childIdx, acc, cur);
+  //             flushIteratepivotLteChildKey0(parent, children, pivots, parentIdx, childrenIdx, childIdx, acc, cur);
+  //             flushIterateRes(parent, children, pivots, parentIdx, childrenIdx + 1, 0, acc + [cur], Kvl(PSA.EmptyPsa(), []));
+  //           }
+  //         }
+  //       } else {
+  //         if PSA.psaElement(child.keys, childIdx as uint64) == PSA.psaElement(parent.keys, parentIdx as uint64) {
+  //           var m := Merge(parent.messages[parentIdx], child.messages[childIdx]);
+  //           if m == IdentityMessage() {
+  //             flushIterateRes(parent, children, pivots, parentIdx + 1, childrenIdx, childIdx + 1, acc, cur);
+  //           } else {
+  //             flushIterateAppendParentAndChild(parent, children, pivots, parentIdx, childrenIdx, childIdx, acc, cur);
+  //             flushIterateRes(parent, children, pivots, parentIdx + 1, childrenIdx, childIdx + 1, acc, append(cur, PSA.psaElement(child.keys, childIdx as uint64), m));
+  //           }
+  //         } else if lt(PSA.psaElement(child.keys, childIdx as uint64), PSA.psaElement(parent.keys, parentIdx as uint64)) {
+  //           flushIterateAppendChild(parent, children, pivots, parentIdx, childrenIdx, childIdx, acc, cur);
+  //           flushIterateRes(parent, children, pivots, parentIdx, childrenIdx, childIdx + 1, acc, append(cur, PSA.psaElement(child.keys, childIdx as uint64), child.messages[childIdx]));
+  //         } else {
+  //           flushIterateAppendParent(parent, children, pivots, parentIdx, childrenIdx, childIdx, acc, cur);
+  //           flushIterateRes(parent, children, pivots, parentIdx + 1, childrenIdx, childIdx, acc, append(cur, PSA.psaElement(parent.keys, parentIdx as uint64), parent.messages[parentIdx]));
+  //         }
+  //       }
+  //     }
+  //   }
+  // }
 
-  lemma flushRes(parent: Kvl, children: seq<Kvl>, pivots: seq<Key>)
-  requires WF(parent)
-  requires forall i | 0 <= i < |children| :: WF(children[i])
-  requires WFBucketListProper(ISeq(children), pivots)
-  ensures var f := flush(parent, children, pivots);
-      && (forall i | 0 <= i < |f| :: WF(f[i]))
-      && ISeq(f) == BucketListFlush(I(parent), ISeq(children), pivots)
-  {
-    reveal_IMap();
-    assert BucketListItemFlush(B(map[]), B(map[]), pivots, 0).b == map[];
-    flushIterateRes(parent, children, pivots, 0, 0, 0, [], Kvl(PSA.EmptyPsa(), []));
-  }
+  // lemma flushRes(parent: Kvl, children: seq<Kvl>, pivots: seq<Key>)
+  // requires WF(parent)
+  // requires forall i | 0 <= i < |children| :: WF(children[i])
+  // requires WFBucketListProper(ISeq(children), pivots)
+  // ensures var f := flush(parent, children, pivots);
+  //     && (forall i | 0 <= i < |f| :: WF(f[i]))
+  //     && ISeq(f) == BucketListFlush(I(parent), ISeq(children), pivots)
+  // {
+  //   reveal_IMap();
+  //   assert BucketListItemFlush(B(map[]), B(map[]), pivots, 0).b == map[];
+  //   flushIterateRes(parent, children, pivots, 0, 0, 0, [], Kvl(PSA.EmptyPsa(), []));
+  // }
 
+  /*
   method Flush(parent: Kvl, children: seq<Kvl>, pivots: seq<Key>)
   returns (f : seq<Kvl>)
   requires WF(parent)
@@ -657,7 +687,8 @@ module KVList {
     flushRes(parent, children, pivots);
     return acc;
   }
-
+   */
+  
   /////////////////////////
   //// Query
   /////////////////////////
@@ -704,6 +735,24 @@ module KVList {
   //// Binary searching
   /////////////////////////
 
+  lemma BinaryLow(keys: seq<Key>, key: Key, i: int)
+    requires IsStrictlySorted(keys)
+    requires 0 <= i < |keys|
+    requires lte(keys[i], key)
+    ensures forall j | 0 <= j < i :: lt(keys[j], key)
+  {
+    reveal_IsStrictlySorted();
+  }
+  
+  lemma BinaryHi(keys: seq<Key>, key: Key, i: int)
+    requires IsStrictlySorted(keys)
+    requires 0 <= i < |keys|
+    requires lte(key, keys[i])
+    ensures forall j | i < j < |keys| :: lt(key, keys[j])
+  {
+    reveal_IsStrictlySorted();
+  }
+  
   method IndexOfFirstKeyGte(kvl: Kvl, key: Key)
   returns (idx: uint64)
   requires WF(kvl)
@@ -722,14 +771,16 @@ module KVList {
     invariant forall i | hi as int <= i < PSA.psaNumStrings(kvl.keys) as int :: lte(key, PSA.psaElement(kvl.keys, i as uint64))
     decreases hi as int - lo as int
     {
-      reveal_IsStrictlySorted();
-
       var mid: uint64 := (lo + hi) / 2;
       var c := cmp(key, PSA.psaElement(kvl.keys, mid));
       if (c > 0) {
         lo := mid + 1;
+        BinaryLow(PSA.I(kvl.keys), key, mid as int);
+        assert forall i | 0 <= i < lo :: PSA.psaElement(kvl.keys, i) == PSA.I(kvl.keys)[i];
       } else {
         hi := mid;
+        BinaryHi(PSA.I(kvl.keys), key, mid as int);
+        assert forall i | lo <= i < PSA.psaNumStrings(kvl.keys) :: PSA.psaElement(kvl.keys, i) == PSA.I(kvl.keys)[i];
       }
     }
 
@@ -760,8 +811,12 @@ module KVList {
       var c := cmp(key, PSA.psaElement(kvl.keys, mid));
       if (c >= 0) {
         lo := mid + 1;
+        BinaryLow(PSA.I(kvl.keys), key, mid as int);
+        assert forall i | 0 <= i < lo :: PSA.psaElement(kvl.keys, i) == PSA.I(kvl.keys)[i];
       } else {
         hi := mid;
+        BinaryHi(PSA.I(kvl.keys), key, mid as int);
+        assert forall i | lo <= i < PSA.psaNumStrings(kvl.keys) :: PSA.psaElement(kvl.keys, i) == PSA.I(kvl.keys)[i];
       }
     }
 
@@ -781,10 +836,23 @@ module KVList {
   {
     reveal_SplitBucketLeft();
     var idx := IndexOfFirstKeyGte(kvl, pivot);
-    left := Kvl(PSA.psaPrefix(kvl.keys, idx), kvl.messages[..idx]);
+    var newkeys := PSA.PsaPrefix(kvl.keys, idx);
+    left := Kvl(newkeys, kvl.messages[..idx]);
 
     reveal_IsStrictlySorted();
-
+    ghost var ikeys := PSA.I(kvl.keys);
+    ghost var inewkeys := PSA.I(newkeys);
+    forall i | 0 <= i < PSA.psaNumStrings(newkeys)
+      ensures PSA.psaElement(newkeys, i) == PSA.psaElement(kvl.keys, i)
+    {
+      calc {
+        PSA.psaElement(newkeys, i);
+        inewkeys[i];
+        ikeys[i];
+        PSA.psaElement(kvl.keys, i);
+      }
+    }
+    
     ghost var a := IMap(left);
     ghost var b := SplitBucketLeft(I(kvl), pivot).b;
 
@@ -817,9 +885,22 @@ module KVList {
   {
     reveal_SplitBucketRight();
     var idx := IndexOfFirstKeyGte(kvl, pivot);
-    right := Kvl(kvl.keys[idx..], kvl.messages[idx..]);
+    var newkeys := PSA.PsaSuffix(kvl.keys, idx);
+    right := Kvl(newkeys, kvl.messages[idx..]);
 
     reveal_IsStrictlySorted();
+    ghost var ikeys := PSA.I(kvl.keys);
+    ghost var inewkeys := PSA.I(newkeys);
+    forall i | 0 <= i < PSA.psaNumStrings(newkeys)
+      ensures PSA.psaElement(newkeys, i) == PSA.psaElement(kvl.keys, idx + i)
+    {
+      calc {
+        PSA.psaElement(newkeys, i);
+        inewkeys[i];
+        ikeys[idx + i];
+        PSA.psaElement(kvl.keys, idx + i);
+      }
+    }
 
     ghost var a := IMap(right);
     ghost var b := SplitBucketRight(I(kvl), pivot).b;
@@ -1032,6 +1113,8 @@ module KVList {
   }*/
 
   method IsWF(kvl: Kvl) returns (b: bool)
+  requires PSA.WF(kvl.keys)
+  requires forall i | 0 <= i < PSA.psaNumStrings(kvl.keys) :: |PSA.psaElement(kvl.keys, i)| <= MaxLen() as int
   requires PSA.psaNumStrings(kvl.keys) as int < 0x1_0000_0000_0000_0000
   requires |kvl.messages| < 0x1_0000_0000_0000_0000
   requires IsStrictlySorted(PSA.I(kvl.keys))
@@ -1040,6 +1123,7 @@ module KVList {
   {
     if PSA.psaNumStrings(kvl.keys)  != |kvl.messages| as uint64
     {
+      assert !WF(kvl);
       return false;
     }
 
@@ -1059,6 +1143,7 @@ module KVList {
     }
     */
 
+    assert WF(kvl);
     return true;
   }
 
@@ -1157,15 +1242,85 @@ module KVList {
   /////////////////////////
 
   function WeightKvl(kvl: Kvl) : int
+    requires PSA.WF(kvl.keys)
+    requires forall i | 0 <= i < PSA.psaNumStrings(kvl.keys) :: |PSA.psaElement(kvl.keys, i)| <= MaxLen() as int
   {
+    var ikeys := PSA.I(kvl.keys);
     WeightKeySeq(PSA.I(kvl.keys)) + WeightMessageSeq(kvl.messages)
   }
 
   function WeightKvlSeq(kvls: seq<Kvl>) : int
+    requires forall i | 0 <= i < |kvls| :: PSA.WF(kvls[i].keys)
+    requires forall j, i | 0 <= j < |kvls| && 0 <= i < PSA.psaNumStrings(kvls[j].keys) :: |PSA.psaElement(kvls[j].keys, i)| <= MaxLen() as int
   {
     if |kvls| == 0 then 0 else WeightKvlSeq(DropLast(kvls)) + WeightKvl(Last(kvls))
   }
 
+  lemma IKeys(kvl: Kvl)
+    requires WF(kvl)
+    ensures I(kvl).b.Keys <= Set(PSA.I(kvl.keys))
+    decreases PSA.psaNumStrings(kvl.keys);
+  {
+    var ikeys := PSA.I(kvl.keys);
+    var ikvl := IMap(kvl);
+    
+    if |ikeys| == 0 {
+    } else {
+      var prekvl := prefix(kvl, |ikeys|-1);
+      WFPrefix(kvl, |ikeys|-1);
+      assert prekvl == Kvl(PSA.psaDropLast(kvl.keys), DropLast(kvl.messages));
+      var lastkey: Key := Last(ikeys);
+      var lastmessage := Last(kvl.messages);
+      reveal_IMap();
+      assert ikvl == IMap(prekvl)[lastkey := lastmessage];
+      IKeys(prekvl);
+    }
+  }
+  
+  lemma LastLargerThanPrefix(kvl: Kvl)
+    requires WF(kvl)
+    requires 0 < PSA.psaNumStrings(kvl.keys)
+    ensures forall k | k in I(prefix(kvl, PSA.psaNumStrings(kvl.keys) as int - 1)).b :: lt(k, PSA.LastElement(kvl.keys))
+    decreases PSA.psaNumStrings(kvl.keys);
+  {
+    var prekvl := Kvl(PSA.psaDropLast(kvl.keys), DropLast(kvl.messages));
+    WFPrefix(kvl, PSA.psaNumStrings(kvl.keys) as int -1);
+    var b := I(prekvl).b;
+
+    var last := PSA.LastElement(kvl.keys);
+    if PSA.psaNumStrings(prekvl.keys) == 0 {
+    } else {
+      var prelast := PSA.LastElement(prekvl.keys);
+      LastLargerThanPrefix(prekvl);
+      var ikeys := PSA.I(kvl.keys);
+      assert last == Last(ikeys);
+      assert prelast == ikeys[|ikeys|-2];
+      IsStrictlySortedImpliesLt(ikeys, |ikeys|-2, |ikeys|-1);
+      forall k | k in b
+        ensures lt(k, last)
+      {
+        IKeys(prekvl);
+        var i :| 0 <= i < |ikeys|-1 && k == ikeys[i];
+        IsStrictlySortedImpliesLte(ikeys, i, |ikeys|-2);
+      }
+    }
+  }
+
+  lemma LastNotInPrefix(kvl: Kvl)
+    requires WF(kvl)
+    requires 0 < PSA.psaNumStrings(kvl.keys)
+    ensures PSA.LastElement(kvl.keys) !in I(prefix(kvl, PSA.psaNumStrings(kvl.keys) as int - 1)).b
+  {
+    LastLargerThanPrefix(kvl);
+    var last := PSA.LastElement(kvl.keys);
+    var pre := I(prefix(kvl, PSA.psaNumStrings(kvl.keys) as int - 1)).b;
+    forall k | k in pre
+      ensures last != k
+    {
+      assert lt(k, last);
+    }
+  }
+  
   lemma kvlWeightEq(kvl: Kvl)
   requires WF(kvl)
   ensures WeightKvl(kvl) == WeightBucket(I(kvl))
@@ -1181,6 +1336,7 @@ module KVList {
         var i := IndexOfKey(Kvl(PSA.psaDropLast(kvl.keys), DropLast(kvl.messages)), PSA.LastElement(kvl.keys));
         reveal_IsStrictlySorted();
       }
+      LastNotInPrefix(kvl);
       WeightBucketInduct(I(Kvl(PSA.psaDropLast(kvl.keys), DropLast(kvl.messages))), PSA.LastElement(kvl.keys), Last(kvl.messages));
       assert WeightKvl(kvl)
           == WeightKvl(Kvl(PSA.psaDropLast(kvl.keys), DropLast(kvl.messages)))
@@ -1206,6 +1362,7 @@ module KVList {
   lemma kvlWeightPrefixLe(kvl: Kvl, j: int)
   requires WF(kvl)
   requires 0 <= j <= PSA.psaNumStrings(kvl.keys) as int
+  ensures WF(prefix(kvl, j))
   ensures WeightKvl(prefix(kvl, j)) <= WeightKvl(kvl);
   decreases PSA.psaNumStrings(kvl.keys) as int
   {
@@ -1249,10 +1406,14 @@ module KVList {
   lemma WeightKvlInduct(kvl: Kvl, j: int)
   requires WF(kvl)
   requires 0 <= j < PSA.psaNumStrings(kvl.keys) as int
+  ensures WF(prefix(kvl, j as int))
+  ensures WF(prefix(kvl, j as int + 1))
   ensures WeightKvl(prefix(kvl, j as int)) +
       WeightKey(PSA.psaElement(kvl.keys, j as uint64)) + WeightMessage(kvl.messages[j])
           == WeightKvl(prefix(kvl, j as int + 1));
   {
+    WFPrefix(kvl, j as int);
+    WFPrefix(kvl, j as int + 1);
     assert DropLast(prefix(kvl, j as int + 1).messages)
         == prefix(kvl, j as int).messages;
     assert PSA.psaDropLast(prefix(kvl, j as int + 1).keys)
@@ -1268,6 +1429,12 @@ module KVList {
     kvlWeightEq(kvl);
     lenKeysLeWeight(kvl);
 
+    forall j | 0 <= j <= PSA.psaNumStrings(kvl.keys) as int
+      ensures WF(prefix(kvl, j as int))
+    {
+      WFPrefix(kvl, j as int);
+    }
+    
     var j: uint64 := 0;
     var w: uint64 := 0;
     while j < PSA.psaNumStrings(kvl.keys) 
@@ -1325,6 +1492,7 @@ module KVList {
   // maximumOpt call, so we wrap it
   function KeySetMax(keys: set<seq<byte>>) : seq<byte>
     requires keys != {}
+    requires forall k | k in keys :: |k| <= MaxLen() as int
   {
     var v: Option<seq<byte>> := maximumOpt(keys);
     v.value
@@ -1333,16 +1501,22 @@ module KVList {
   
   lemma lastIsMax(kvl: Kvl)
   requires WF(kvl)
-  requires PSA.psaNumStrings(kvl.keys) as int > 0
+  requires 0 < PSA.psaNumStrings(kvl.keys) as int
+  ensures I(kvl).b.Keys != {}
   ensures KeySetMax(I(kvl).b.Keys) == PSA.LastElement(kvl.keys)
   {
     Imaps(kvl, PSA.psaNumStrings(kvl.keys) as int - 1);
     assert PSA.LastElement(kvl.keys) in IMap(kvl).Keys;
+    LastLargerThanPrefix(kvl);
+    var ikeys := PSA.I(kvl.keys);
+    var last := PSA.LastElement(kvl.keys);
+    assert last == Last(ikeys);
     forall key | key in IMap(kvl).Keys
     ensures lte(key, PSA.LastElement(kvl.keys))
     {
       var i := IndexOfKey(kvl, key);
-      reveal_IsStrictlySorted();
+      assert ikeys[i] == key;
+      IsStrictlySortedImpliesLte(ikeys, i, |ikeys|-1);
     }
   }
 
@@ -1353,11 +1527,7 @@ module KVList {
   ensures PSA.LastElement(kvl.keys) !in IMap(Kvl(PSA.psaDropLast(kvl.keys), DropLast(kvl.messages)));
   {
     WFPrefix(kvl, PSA.psaNumStrings(kvl.keys) as int - 1);
-    if PSA.LastElement(kvl.keys) in IMap(Kvl(PSA.psaDropLast(kvl.keys), DropLast(kvl.messages))) {
-      var i := IndexOfKey(Kvl(PSA.psaDropLast(kvl.keys), DropLast(kvl.messages)), PSA.LastElement(kvl.keys));
-      assert PSA.psaElement(kvl.keys, i as uint64) == PSA.LastElement(kvl.keys);
-      reveal_IsStrictlySorted();
-    }
+    LastNotInPrefix(kvl);
   }
 
   lemma I_injective(kvl1: Kvl, kvl2: Kvl)
